Fix AST.

Practical_Foundation_of_Programming_Languages/PLT.v
@@ -16,53 +16,116 @@ Inductive ihlist { F : Type -> Type } : list Type -> Type :=
 
 Implicit Arguments ihlist[].
 
-Definition operator := list Type.
+Definition operator (S : Type) := list Type.
+Definition variable (S : Type) := unit.
+
+Inductive Pos A : A -> list A -> Type :=
+| Pos_fst : forall a l, Pos a (a :: l)
+| Pos_skip : forall a a' l, Pos a' l -> Pos a' (a :: l).
 
 Inductive AXs
   { S : set Type }
-    { Os : forall s, contain S s -> list operator }
-    { Xs : forall s, contain S s -> list s } : Type -> Type :=
-| XAXs : forall s (c : contain S s)(s' : s), In s' (Xs s c) -> AXs s
-| OAXs : forall s (c : contain S s)(op : operator), In op (Os s c) -> 
+    { Os : forall s, contain S s -> list (operator s) }
+    { Xs : forall s, contain S s -> list (variable s) } : Type -> Type :=
+| XAXs : forall s (c : contain S s)(va : variable s), Pos va (Xs s c) -> AXs s
+| OAXs : forall s (c : contain S s)(op : operator s), Pos op (Os s c) -> 
     ihlist (fun s' => AXs s') op -> AXs s.
 
 Implicit Arguments AXs[].
 Implicit Arguments OAXs[s c op S Os Xs].
-Implicit Arguments XAXs[s c s' S Os Xs].
+Implicit Arguments XAXs[s c va S Os Xs].
 Implicit Arguments ihcons[T L F].
 
+Definition subst { S S' } (s : S)(Heq : S ~= S') : {s' : S' | s ~= s' }.
+  subst.
+  exists s.
+  trivial.
+Defined.
+
+Theorem subst_eq : forall S (eq : S ~= S)(s : S), JMeq s (proj1_sig(subst s eq)).
+  intros.
+  destruct (subst s eq).
+  trivial.
+Qed.
+
+Definition adjoin { S : set Type } (Xs : forall s, contain S s -> list (variable s))
+  { s : Type } { sdec : forall t, { s = t } + { s <> t } } (c : contain S s) (v : variable s) : 
+    forall s' (c' : contain S s'),
+      { ls : list (variable s') | 
+          (forall (eq : s = s'), ls = v :: (Xs _ c)) /\
+          (s' <> s -> ls = Xs _ c') }.
+  intros.
+  destruct (sdec s').
+  subst.
+  exists (v :: (Xs _ c)).
+  intuition.
+  exists (Xs s' c').
+  intuition.
+Defined.
+
 Inductive ihlist_forall (F : Type -> Type) { P : forall T, F T -> Type } : 
-  forall L, ihlist F L -> Prop :=
+  forall L, ihlist F L -> Type :=
 | Forall_ihnil : ihlist_forall ihnil
 | Forall_ihcons : forall (l : list Type)(L : ihlist F l)(T : Type)(t : F T), 
     P T t -> ihlist_forall L -> ihlist_forall (ihcons t L).
 
 Implicit Arguments ihlist_forall[F].
 
-Fixpoint Induction S Os Xs (P : forall T, AXs S Os Xs T -> Type)
-  (FX : forall s (c : contain S s)(s' : s)(i : In s' (Xs s c)), P s (XAXs i))
-  (FO : forall s (c : contain S s)(op : operator)(i : In op (Os s c))
+Fixpoint AST_rect S Os Xs (P : forall T, AXs S Os Xs T -> Type)
+  (FX : forall s (c : contain S s)(s' : variable s)(i : Pos s' (Xs s c)), P s (XAXs i))
+  (FO : forall s (c : contain S s)(op : operator s)(i : Pos op (Os s c))
     (l : ihlist (fun s' => AXs S Os Xs s') op), 
       ihlist_forall (fun t ax => P t ax) op l -> P s (OAXs i l))
   T (AX : AXs S Os Xs T) : P T AX.
   destruct AX;
   trivial.
   apply FO.
-  clear i.
-  induction i0;
-  constructor.
-  apply Induction;
+  clear p.
+  induction i;
+  constructor;
+  try apply AST_rect;
   trivial.
-  apply IHi0.
 Defined.
 
-Inductive isnat : Type -> Prop := isnat_nat : isnat nat.
+Fixpoint AST_size S Os Xs T (ast : AXs S Os Xs T) : nat :=
+  match ast with
+  | XAXs _ _ _ _ => 1
+  | OAXs _ _ _ _ il => 1 +
+      ((fix ilind t (l : ihlist _ t) : nat := 
+        match l with
+        | ihnil => 0
+        | ihcons _ _ a l' => AST_size a + ilind _ l'
+        end) _ il)
+  end.
 
-Definition plus : list Type := (@cons Type nat (@cons Type nat nil)).
-
-Definition natast := AXs isnat (fun _ _ => [plus]) (fun _ _ => nil) nat.
-
-Goal natast -> False.
+Theorem ast_size : forall S Os Xs T (ast : AXs S Os Xs T), { n | n = AST_size ast }.
   intros.
-  apply (Induction X).
-Qed.
+  refine (@AST_rect S Os Xs (fun _ ast' => {n : nat | n = AST_size ast'}) _ _ T ast);
+  intros;
+  simpl in *.
+  eauto.
+  clear i.
+  induction X.
+  eauto.
+  destruct p, IHX.
+  exists (x + x0).
+  subst.
+  auto.
+Defined.
+
+Extraction ast_size. (*Testing if AST_rect is useful*)
+
+Inductive subeq : forall S Xs Os s s'(x : variable s)(c : contain S s)(a : AXs S Os (adjoin Xs _ x _ c) Os s')(b : AXs S Xs Os s'), Prop :=.
+
+Variables are given meaning by substitution. If x is a variable of sort s, a ∈ A[X , x ] s 0 ,
+and b ∈ A[X ] s , then [ b/x ] a ∈ A[X ] s 0 is defined to be the result of substituting b for
+every occurrence of x in a. The ast a is called the target, and x is called the subject, of the
+substitution. Substitution is defined by the following equations:
+1. [ b/x ] x = b and [ b/x ] y = y if x 6 = y.
+For example, we may check that
+ew
+2. [ b/x ] o(a 1 ; . . . ;a n ) = o( [ b/x ] a 1 ; . . . ; [ b/x ] a n ).
+[ num[2]/x ] plus(x; num[3]) = plus(num[2]; num[3]).
+We may prove by structural induction that substitution on ast’s is well-defined.
+Theorem 1.1. If a ∈ A[X , x ] , then for every b ∈ A[X ] there exists a unique c ∈ A[X ] such that
+[ b/x ] a = c
